memabs/SemDef.v
@@ -1,48 +1,209 @@
 Require Import Coqlib.
 Require Import LanguageInterface Events Globalenvs Values Memory AST Errors Smallstep.
 Require Import Clight Ctypes Cop.
+Require Import CKLR.
 Require Import Coherence CompCertSem Bigstep.
 
-(* Define a language interface with memory abstracted out *)
-Record d_query :=
-  dq {
-      dq_vf: val;
-      dq_sg: signature;
-      dq_args: list val;
-    }.
-Record d_reply :=
-  dr {
-      dr_retval: val;
-    }.
-Canonical Structure li_d :=
+Definition sem_coherence {liA liB} (L: semantics liA liB) :=
+  forall se t1 e1 t2 e2,
+    lts_lmaps (L se) t1 e1 ->
+    lts_lmaps (L se) t2 e2 ->
+    @coh (!liA --o liB) (t1, e1) (t2, e2).
+
+Lemma determ_coh {liA liB} (L: semantics liA liB):
+  determinate L -> sem_coherence L.
+Proof.
+  intros HL.
+  intros se eas [qb rb] eas' [qb' rb'] lmap lmap' coheas. cbn.
+  split.
+  - split; auto.
+    intros <-.
+    inversion lmap as [? ? ? ? valid_q init_q transition_q]. subst.
+    inversion lmap' as [? ? ? ? valid_q' init_q' transition_q']. subst.
+    determ_solve (sd_initial_determ (HL se)).
+    exploit @trace_determ. exact HL.
+    exact coheas. exact transition_q. exact transition_q'.
+    intuition.
+  - intros h. inv h.
+    inversion lmap as [? ? ? ? valid_q init_q transition_q]. subst.
+    inversion lmap' as [? ? ? ? valid_q' init_q' transition_q']. subst.
+    determ_solve (sd_initial_determ (HL se)).
+    exploit @trace_determ. exact HL.
+    exact coheas. exact transition_q. exact transition_q'.
+    intuition.
+Qed.
+
+(* A semantics embedding with deterministic condition relaxed *)
+Section SEMANTICS.
+  Context {liA liB} (L : semantics liA liB) (HL : sem_coherence L).
+  Program Definition compcerto_lmap' se : !liA --o liB :=
+    {|
+    has '(t, u) := lts_lmaps (L se) t u;
+    |}.
+  Next Obligation.
+    intros Hcoh. exploit HL. apply H. apply H0. apply Hcoh.
+    now cbn.
+  Qed.
+End SEMANTICS.
+
+(* A coh semantics with valid_query predicate; eventually the semantics should
+   also include a predicate to make sure outgoing calls are in scope *)
+Record coh_semantics (liA liB: language_interface): Type :=
+  {
+  vq: query liB -> bool;            (* valid_query *)
+  lf:> !liA --o liB;            (* linear func *)
+  Hvq: forall t q r, has lf (t, (q, r)) -> vq q = true;
+  }.
+Record coh_refinement' {liA liB1 liB2} (ccB: callconv liB1 liB2) (wB: ccworld ccB)
+       (Σ1: coh_semantics liA liB1) (Σ2: coh_semantics liA liB2) : Prop :=
+  {
+  coh_vq_ref: forall q1 q2, match_query ccB wB q1 q2 -> vq _ _ Σ1 q1 = vq _ _ Σ2 q2;
+  coh_lf_ref: forall q1 q2 r1 t, has Σ1 (t, (q1, r1)) ->
+                            match_query ccB wB q1 q2 ->
+                            exists r2, has Σ2 (t, (q2, r2)) /\
+                                  match_reply ccB wB r1 r2;
+  }.
+Definition coh_refinement {liA liB1 liB2: language_interface}
+           (ccB: callconv liB1 liB2)
+           (Σ1: Genv.symtbl -> coh_semantics liA liB1)
+           (Σ2: Genv.symtbl -> coh_semantics liA liB2) sk : Prop :=
+  forall se1 se2 wB,
+    match_senv ccB wB se1 se2 ->
+    Genv.valid_for sk se1 ->
+    coh_refinement' ccB wB (Σ1 se1) (Σ2 se2).
+
+Section COH_UNSEM.
+  Context {liA liB : language_interface} (Σ : coh_semantics liA liB).
+  Definition coh_lts : lts liA liB UnSem.state :=
+    {|
+    Smallstep.step _ := UnSem.step;
+    Smallstep.valid_query q := vq _ _ Σ q;
+    Smallstep.initial_state := UnSem.initial_state Σ;
+    Smallstep.at_external := UnSem.at_external;
+    Smallstep.after_external := UnSem.after_external;
+    Smallstep.final_state := UnSem.final_state;
+    Smallstep.globalenv := tt;
+    |}.
+End COH_UNSEM.
+(* Anti-embedding coh semantics into lts *)
+Definition coh_unsem {liA liB : language_interface} skel
+           (Σ : _ -> coh_semantics liA liB) :=
   {|
-  query := d_query;
-  reply := d_reply;
-  entry := dq_vf;
+  Smallstep.skel := skel;
+  Smallstep.activate se := coh_lts (Σ se);
   |}.
-Inductive q_rel: query li_d -> query li_c -> mem -> Prop:=
-| q_rel_intro:
-    forall vf sg args m,
-      q_rel ({|dq_vf:=vf;dq_sg:=sg;dq_args:=args|})
-            ({|cq_vf:=vf;cq_sg:=sg;cq_args:=args;cq_mem:=m|}) m.
-Inductive r_rel: reply li_d -> reply li_c -> mem -> Prop:=
-  r_rel_intro:
-    forall ret m,
-      r_rel ({|dr_retval:=ret|})
-            ({|cr_retval:=ret;cr_mem:=m|}) m.
-Inductive qr_rel_list: list (query li_d * reply li_d) -> list (query li_c * reply li_c) -> Prop:=
-| qr_rel_nil: qr_rel_list nil nil
-| qr_rel_cons:
-    forall dq dr cq cr ds cs m m',
-      q_rel dq cq m ->
-      r_rel dr cr m' ->
-      qr_rel_list ds cs ->
-      qr_rel_list ((dq, dr)::ds) ((cq, cr)::cs).
-Inductive li_rel: (query li_d * reply li_d) -> (query li_c * reply li_c) -> Prop:=
+(* Embedding lts semantics into coh *)
+Program Definition lts_sem {liA liB: language_interface}
+        (L: semantics liA liB) (HL: sem_coherence L) se: coh_semantics liA liB :=
+  {|
+  vq := valid_query (L se);
+  lf := compcerto_lmap' L HL se;
+  |}.
+Next Obligation.
+  intros. now inv H.
+Qed.
+
+(* The Galois Connection with calling conventions on incoming queries and
+   replies. The proof hasn't been figured out. 1. sem_coherence is too weak;
+   2. match_states should take the cc into consideration *)
+Section GC_CC.
+  Context {liA liB : language_interface}.
+  Context (Σ : Genv.symtbl -> coh_semantics liA liB).
+  Context (L : semantics liA liB) (HL : sem_coherence L).
+
+  Inductive match_states se : nat -> UnSem.state -> Smallstep.state L -> Prop :=
+    match_states_intro (b : bool) (σ : UnSem.trace_set) (s : Smallstep.state L) :
+      (forall t r, has σ (t, r) -> lts_trace (L se) b s t r) ->
+      match_states se (Nat.b2n b) (b, σ) s.
+
+  Definition measure : (@UnSem.state liA liB) -> nat :=
+    fun '(b, _) => if b then 1%nat else 0%nat.
+
+  Let sk := skel L.
+  Lemma sem_unsem_gc cc:
+    coh_refinement cc Σ (lts_sem L HL) sk <->
+    forward_simulation cc_id cc (coh_unsem sk Σ) L.
+  Proof.
+  Admitted.
+End GC_CC.
+
+(* A simplified version of GC without calling convertions and deterministic
+   condition is assumed *)
+Section GC.
+End GC.
+
+(* A language interface without memory involved *)
+Record d_query :=
+  dq { dq_vf: val;
+       dq_sg: signature;
+       dq_args: list val; }.
+Record d_reply :=
+  dr { dr_retval: val; }.
+Canonical Structure li_d :=
+  {| query := d_query;
+     reply := d_reply;
+     entry := dq_vf; |}.
+(* A relation that allows arguments in C language interface to be more
+   defined than those in abstract language interface *)
+Inductive q_rel': query li_d -> query li_c -> mem -> Prop:=
+| q_rel'_intro:
+    forall vf sg args args' m,
+      list_rel Val.lessdef args args' ->
+      q_rel' ({|dq_vf:=vf;dq_sg:=sg;dq_args:=args|})
+             ({|cq_vf:=vf;cq_sg:=sg;cq_args:=args';cq_mem:=m|}) m.
+Definition r_with_mem (r: reply li_d) m: reply li_c :=
+  match r with
+    {|dr_retval:=ret|} => ({|cr_retval:=ret;cr_mem:=m|})
+  end.
+Definition q_with_mem (q: query li_d) m: query li_c :=
+  match q with
+    {|dq_vf:=vf;dq_sg:=sg;dq_args:=args|} =>
+    {|cq_vf:=vf;cq_sg:=sg;cq_args:=args;cq_mem:=m|}
+  end.
+Inductive vals_defined: list val -> Prop :=
+| vals_defined_nil: vals_defined nil
+| vals_defined_cons: forall v vs,
+    v <> Vundef -> vals_defined vs ->
+    vals_defined (v::vs).
+Definition query_defined (q: query li_d): Prop :=
+  match q with
+    {|dq_vf:=_;dq_sg:=_;dq_args:=args|} => vals_defined args
+  end.
+Lemma defined_query_with_mem q q' m:
+  query_defined q -> q_rel' q q' m ->
+  q' = q_with_mem q m.
+Proof.
+  intros. inv H0. cbn in *.
+  f_equal. symmetry. revert args' H1.
+  induction H.
+  intros. inv H1. auto. intros. inv H1. f_equal.
+  inv H4; easy. apply IHvals_defined. auto.
+Qed.
+(* Inductive q_rel: query li_d -> query li_c -> mem -> Prop:= *)
+(* | q_rel_intro: *)
+(*     forall vf sg args m, *)
+(*       q_rel ({|dq_vf:=vf;dq_sg:=sg;dq_args:=args|}) *)
+(*             ({|cq_vf:=vf;cq_sg:=sg;cq_args:=args;cq_mem:=m|}) m. *)
+(* Inductive r_rel: reply li_d -> reply li_c -> mem -> Prop:= *)
+(*   r_rel_intro: *)
+(*     forall ret m, *)
+(*       r_rel ({|dr_retval:=ret|}) *)
+(*             ({|cr_retval:=ret;cr_mem:=m|}) m. *)
+(* Inductive qr_rel_list: list (query li_d * reply li_d) -> list (query li_c * reply li_c) -> Prop:= *)
+(* | qr_rel_nil: qr_rel_list nil nil *)
+(* | qr_rel_cons: *)
+(*     forall dq dr cq cr ds cs m m', *)
+(*       q_rel dq cq m -> *)
+(*       r_rel dr cr m' -> *)
+(*       qr_rel_list ds cs -> *)
+(*       qr_rel_list ((dq, dr)::ds) ((cq, cr)::cs). *)
+Inductive li_rel: token li_d -> token li_c -> Prop:=
 | rel_intro:
     forall vf sg args ret m,
-      li_rel ({|dq_vf:=vf;dq_sg:=sg;dq_args:=args|}, {|dr_retval:=ret|})
-             ({|cq_vf:=vf;cq_sg:=sg;cq_args:=args;cq_mem:=m|}, {|cr_retval:=ret;cr_mem:=m|}).
+      li_rel ({|dq_vf:=vf;dq_sg:=sg;dq_args:=args|},
+              {|dr_retval:=ret|})
+             ({|cq_vf:=vf;cq_sg:=sg;cq_args:=args;cq_mem:=m|},
+              {|cr_retval:=ret;cr_mem:=m|}).
 
 Program Definition li_dc: li_d --o li_c :=
   {|
@@ -72,34 +233,35 @@ Next Obligation.
   split. inversion Hr. subst. apply H5. auto.
   intro. exploit Hl. f_equal. auto. apply app_inv_head.
 Qed.
-
+(* This module aims to define C @ Σ, where C is a Clight program and Σ is an
+   underlay specification within coherent spaces. The composed transition system
+   behaves like C with external calls interpreted by Σ. We first define a
+   general version L @ Σ for arbitrary transition system L and later refine it
+   to C semantics *)
 Module Abs.
   Section ABS_SEMANTICS.
     (* the linked system has type liA ->> liD *)
-    Context {liA liB liC liD: language_interface} (Σ: Genv.symtbl -> !liA --o !liB) (C: semantics liC liD).
-    Variable li_rel: (query liB * reply liB) -> (query liC * reply liC) -> Prop.
+    Context {liA liB liC liD: language_interface}
+            (Σ: Genv.symtbl -> !liA --o !liB) (L: semantics liC liD).
+    Variable li_rel: token liB -> token liC -> Prop.
     Variable se: Genv.symtbl.
 
     Variant state : Type :=
-    | st (s: Smallstep.state C) (σ: !liA --o !liB)
+    | st (s: Smallstep.state L) (σ: !liA --o !liB)
     (* s and σ constitute the state after the external call *)
-    | ext (s: Smallstep.state C) (t: list (token liA)) (σ: !liA --o !liB).
+    | ext (s: Smallstep.state L) (t: list (token liA)) (σ: !liA --o !liB).
 
     Inductive step: state -> trace -> state -> Prop :=
     | step_internal: forall s s' t σ,
-        Step (C se) s t s' ->
+        Step (L se) s t s' ->
         step (st s σ) t (st s' σ)
     | step_at_external: forall s s' qa ra qb rb σ w,
-        Smallstep.at_external (C se) s qb ->
-        Smallstep.after_external (C se) s rb s' ->
-        (* (w, r) may not be the "right" execution. In other words, [next σ w q
-           r] might be empty.  But that's fine because it's still related to s
-           per correctness *)
+        (* Upon an external query, the memory is dropped from the query. The
+           system proceeds with the same memory for whatever reply from Σ *)
+        Smallstep.at_external (L se) s qb ->
+        Smallstep.after_external (L se) s rb s' ->
+        (* [exec σ q w r] introduces non-determinism *)
         exec σ qa w ra ->
-        (* drop the memory and make a query. take the reply and attach the same
-        memory to it *)
-        (* this can be further refined by giving the reply a new memory as long
-        as it's larger than the old one *)
         li_rel (qa, ra) (qb, rb) ->
         step (st s σ) E0 (ext s' w (next σ w qa ra))
     | step_after_external: forall s σ,
@@ -107,7 +269,7 @@ Module Abs.
 
     Inductive initial_state: query liD -> state -> Prop :=
     | initial_state_intro: forall q s,
-        Smallstep.initial_state (C se) q s ->
+        Smallstep.initial_state (L se) q s ->
         initial_state q (st s (Σ se)).
 
     Inductive at_external: state -> query liA -> Prop :=
@@ -119,46 +281,214 @@ Module Abs.
 
     Inductive final_state: state -> reply liD -> Prop :=
     | final_state_intro: forall s r σ,
-        Smallstep.final_state (C se) s r ->
+        Smallstep.final_state (L se) s r ->
         final_state (st s σ) r.
 
     Definition lts : lts liA liD state :=
       {|
       Smallstep.step _ := step;
-      Smallstep.valid_query := Smallstep.valid_query (C se);
+      Smallstep.valid_query := Smallstep.valid_query (L se);
       Smallstep.initial_state := initial_state;
       Smallstep.at_external := at_external;
       Smallstep.after_external := after_external;
       Smallstep.final_state := final_state;
-      Smallstep.globalenv := Smallstep.globalenv (C se);
+      Smallstep.globalenv := Smallstep.globalenv (L se);
       |}.
   End ABS_SEMANTICS.
   Definition semantics {liA liB liC liD: language_interface}
-             skel li_rel (Σ: Genv.symtbl -> !liA --o !liB) (C: Smallstep.semantics liC liD) :=
+             skel li_rel (Σ: Genv.symtbl -> !liA --o !liB)
+             (L: Smallstep.semantics liC liD) :=
     {|
     Smallstep.skel := skel;
-    Smallstep.activate se := lts Σ C li_rel se;
+    Smallstep.activate se := lts Σ L li_rel se;
     |}.
-  Definition c_semantics sk (C: Clight.program) (Σ: Genv.symtbl -> !li_d --o !li_d) : Smallstep.semantics li_d li_c :=
+  Definition c_semantics sk (C: Clight.program)
+             (Σ: Genv.symtbl -> !li_d --o !li_d): Smallstep.semantics li_d li_c :=
     semantics sk li_rel Σ (semantics1 C).
 End Abs.
 
+(* 〚L @ Σ〛 Embedding of a mixed semantics into coherent spaces *)
+Section ABS_EMBED.
+  Context {liA liB: language_interface} (Σ: Genv.symtbl -> !liA --o !liB).
+  Context {liC liD: language_interface} (L: semantics liC liD) (HL: determinate L).
+  Variable li_rel: token liB -> token liC -> Prop.
+
+  Definition li_rel_determ : Prop :=
+    forall qx rx qy ry qx' rx' qy' ry',
+      li_rel (qx, rx) (qy, ry) ->
+      li_rel (qx', rx') (qy', ry') ->
+      qy = qy' -> qx = qx' /\ (rx = rx' -> ry = ry').
+
+  Hypothesis lr_determ: li_rel_determ.
+
+  Lemma star_ext_state se σ s w ws t s':
+    Star (Abs.lts Σ L li_rel se) (Abs.ext L s (w :: ws) σ) t s' ->
+    s' = Abs.ext L s (w :: ws) σ.
+  Proof.
+    intros Hstar.
+    inv Hstar. reflexivity. inv H.
+  Qed.
+
+  Lemma trace_prefix se s w σ t r:
+    lts_trace (Abs.lts Σ L li_rel se) false (Abs.ext L s w σ) t r ->
+    exists t', t = w ++ t'.
+  Proof.
+    revert t. induction w.
+    - intros. eexists. reflexivity.
+    - intros t Hlts.
+      inv Hlts. inv H. inv H. inv H0.
+      inv H1. destruct w.
+      + eexists. cbn. reflexivity.
+      + eapply star_ext_state in H.
+        subst. exploit IHw. eauto.
+        intros [? ?]. eexists.
+        rewrite <- app_comm_cons. f_equal. eauto.
+  Qed.
+
+  (* L determ + Σ coherence = L @ Σ coherence *)
+  Let LΣ := Abs.semantics (skel L) li_rel Σ L.
+  Lemma LΣ_coh: sem_coherence LΣ.
+  Proof.
+    intros se bot_tr' [q' r'] bot_tr [q r] H H0. cbn.
+    intros Hcoh. assert (q' = q -> r' = r /\ bot_tr' = bot_tr).
+    {
+      intros ->. inv H. inv H0. inv H5. inv H7.
+      exploit (sd_initial_determ (HL se)). apply H. apply H0.
+      intros ->. clear H H0 H2 H3.
+      revert bot_tr Hcoh H8. induction H6.
+      - intros tr Hcoh Hlts.
+        inv Hlts. apply IHlts_trace. auto.
+        replace s' with s'0. auto.
+        clear - lr_determ Hcoh HL H H0 H1 H6. revert s'0 H0 H1.
+        induction H.
+        + intros. inv H0; auto.
+          inv H6.
+          * inv H0. inv H.
+            -- exploit (sd_final_nostep (HL se)); eauto. easy.
+            -- exploit (sd_final_noext (HL se)); eauto. easy.
+          * inv H0. inv H.
+        + intros. specialize (IHstar H6).
+          inv H2.
+          * inv H3.
+            -- inv H1. inv H.
+               ** exploit (sd_final_nostep (HL se)); eauto. easy.
+               ** exploit (sd_final_noext (HL se)); eauto. easy.
+            -- inv H1. inv H.
+          * inv H.
+            -- inv H4.
+               ** exploit (sd_determ (HL se)). apply H1. apply H10.
+                  exploit (sd_traces (HL se)). apply H1.
+                  exploit (sd_traces (HL se)). apply H10. intros l1 l2.
+                  intros [Hmt Ht].
+                  assert (t1 = t3 /\ t2 = t4).
+                  destruct t1. inv Hmt. split; auto.
+                  destruct t1. 2: { simpl in l2. try omegaContradiction. }
+                  destruct t3. inv Hmt. destruct t3.
+                  2: { simpl in l1. try omegaContradiction. }
+                  simpl in H7. inv H7. split; auto.
+                  exploit Ht. apply H. intros <-.
+                  destruct H as [<- <-].
+                  eapply IHstar. auto. auto.
+               ** exploit (sd_at_external_nostep (HL se)); eauto. easy.
+            -- inv H4.
+               ** exploit (sd_at_external_nostep (HL se)); eauto. easy.
+               ** exploit (sd_at_external_determ (HL se)). apply H1. apply H11.
+                  intros <-. inv H8. inv H13.
+                  exploit lr_determ. apply H9. apply H16. auto.
+                  intros [<- Hr].
+                  destruct w; destruct w0.
+               ++ pose proof (has_coh _ _ _ _ H H4).
+                  cbn in H8. exploit H8. constructor.
+                  intros [Hl Hqr]. inv Hl.
+                  cbn in H15. exploit (proj2 H15). auto. intros <-.
+                  exploit Hr. auto. intros <-.
+                  exploit (sd_after_external_determ (HL se)). apply H2. apply H12.
+                  intros <-. simpl in H7. subst. apply IHstar. auto. auto.
+               ++ pose proof (has_coh _ _ _ _ H H4).
+                  cbn in H8. exploit H8. constructor.
+                  intros [Hl Hqr]. inv Hl.
+                  cbn in H15. exploit (proj2 H15). auto. intros <-.
+                  exploit Hqr. constructor. intros. easy.
+               ++ pose proof (has_coh _ _ _ _ H H4).
+                  cbn in H8. exploit H8. constructor.
+                  intros [Hl Hqr]. inv Hl.
+                  cbn in H15. exploit (proj2 H15). auto. intros <-.
+                  exploit Hqr. constructor. intros. easy.
+               ++ pose proof (has_coh _ _ _ _ H H4).
+                  cbn in H8. exploit H8.
+                  exploit star_ext_state. apply H0. intros ->.
+                  exploit star_ext_state. apply H5. intros ->.
+                  exploit trace_prefix. apply H6. intros [? ->].
+                  exploit trace_prefix. apply H3. intros [? ->].
+                  eapply prefix_coh. eauto.
+                  intros [Hl Hqr]. inv Hl.
+                  cbn in H15. exploit (proj2 H15). auto.
+                  intros <-. exploit Hr. auto. intros <-.
+                  exploit (sd_after_external_determ (HL se)). apply H2. apply H12.
+                  intros <-. simpl in H7. subst.
+                  exploit Hqr. auto. intros. inv H7.
+                  apply IHstar. auto. auto.
+            -- inv H4. simpl in H7. subst.
+               apply IHstar. auto. auto.
+      - intros tr Hcoh Hlts. inv Hcoh.
+        + inv H. inv Hlts.
+          * inv H. exploit (sd_final_determ (HL se)). apply H0. apply H4. easy.
+          * inv H.
+        + inv Hlts. inv H. inv H0.
+          exploit (sd_final_determ (HL se)). apply H1. apply H4. easy.
+      - intros tr Hcoh Hlts.
+        inv Hcoh.
+        + inv Hlts. inv H1. inv H.
+        + destruct b as [q' r'].
+          inv Hlts. inv H. inv H7.
+          inv H0. inv H9. exploit H5. auto.
+          intros Hcoh'.
+          exploit IHlts_trace; eauto. intros [<- <-]. easy.
+    }
+    split. split; auto. apply H1. intros. apply H1. inv H2. auto.
+  Qed.
+
+  Program Definition mix_sem se: coh_semantics liA liD :=
+    {|
+    vq := valid_query (L se);
+    lf := compcerto_lmap' LΣ LΣ_coh se;
+    |}.
+  Next Obligation.
+    inv H. apply H2.
+  Qed.
+End ABS_EMBED.
+Lemma determ_li_dc: li_rel_determ li_rel.
+Proof.
+  unfold li_rel_determ.
+  intros. inv H. inv H0.
+  split. auto. intros. inv H. auto.
+Qed.
+Definition c_mix_sem p (Σ : Genv.symtbl -> !li_d --o !li_d) se :=
+  mix_sem Σ (semantics1 p) (clight_determinate p)
+          li_rel determ_li_dc se.
+
+(* This module aims to define C ⊕ p, where C and p are both Clight program. The
+   composition in not commutative in the sense that the only interactive between
+   C and p is C make calls defined within the scope p. We first define L ⊕ σ,
+   where L is arbitrary transition system and σ can be thought as a form of
+   big-step semantics, which will be instantiated to C big-step semantics *)
 Module Impl.
   Section IMPL_SEMANTICS.
-    Context {liA liB liC: language_interface} (σ: Genv.symtbl -> !liA --o liB) (C: semantics liB liC).
+    Context {liA liB liC: language_interface}
+            (σ: Genv.symtbl -> !liA --o liB) (L: semantics liB liC).
     Variable se: Genv.symtbl.
 
     Variant state :=
-    | st (s: Smallstep.state C)
-    | ext (s: Smallstep.state C) (t: list (token liA)).
+    | st (s: Smallstep.state L)
+    | ext (s: Smallstep.state L) (t: list (token liA)).
 
     Inductive step: state -> trace -> state -> Prop :=
     | step_internal: forall s s' t,
-        Step (C se) s t s' ->
+        Step (L se) s t s' ->
         step (st s) t (st s')
     | step_at_external: forall s s' q r t,
-        Smallstep.at_external (C se) s q ->
-        Smallstep.after_external (C se) s r s' ->
+        Smallstep.at_external (L se) s q ->
+        Smallstep.after_external (L se) s r s' ->
         has (σ se) (t, (q, r)) ->
         step (st s) E0 (ext s' t)
     | step_after_external: forall s,
@@ -166,7 +496,7 @@ Module Impl.
 
     Inductive initial_state: query liC -> state -> Prop :=
     | initial_state_intro: forall q s,
-        Smallstep.initial_state (C se) q s ->
+        Smallstep.initial_state (L se) q s ->
         initial_state q (st s).
 
     Inductive at_external: state -> query liA -> Prop :=
@@ -178,26 +508,166 @@ Module Impl.
 
     Inductive final_state: state -> reply liC -> Prop :=
     | final_state_intro: forall s r,
-        Smallstep.final_state (C se) s r ->
+        Smallstep.final_state (L se) s r ->
         final_state (st s) r.
 
     Definition lts : lts liA liC state :=
       {|
       Smallstep.step _ := step;
-      Smallstep.valid_query := Smallstep.valid_query (C se);
+      Smallstep.valid_query := Smallstep.valid_query (L se);
       Smallstep.initial_state := initial_state;
       Smallstep.at_external := at_external;
       Smallstep.after_external := after_external;
       Smallstep.final_state := final_state;
-      Smallstep.globalenv := Smallstep.globalenv (C se);
+      Smallstep.globalenv := Smallstep.globalenv (L se);
       |}.
   End IMPL_SEMANTICS.
   Definition semantics {liA liB liC: language_interface}
-             skel (σ: Genv.symtbl -> !liA --o liB) (C: Smallstep.semantics liB liC) :=
+             skel (σ: Genv.symtbl -> !liA --o liB)
+             (L: Smallstep.semantics liB liC) :=
     {|
     Smallstep.skel := skel;
-    Smallstep.activate se := lts σ C se;
+    Smallstep.activate se := lts σ L se;
     |}.
-  Definition c_semantics sk (C: Clight.program) (p: Clight.program): Smallstep.semantics li_d li_c :=
+  Definition c_semantics sk (C: Clight.program) (p: Clight.program):
+    Smallstep.semantics li_d li_c :=
     semantics sk (fun se => clight_bigstep p se @ !li_dc) (semantics1 C).
 End Impl.
+
+(* 〚C ⊕ p〛Embedding of the composed semantics *)
+Section IMPL_EMBED.
+
+  Context {liA liB liC: language_interface}
+          (σ: Genv.symtbl -> !liA --o liB) (L: semantics liB liC)
+          (HL: determinate L).
+
+  Lemma star_ext_state' se s w ws t s':
+    Star (Impl.lts σ L se) (Impl.ext L s (w :: ws)) t s' ->
+    s' = @Impl.ext _ liB liC L s (w :: ws).
+  Proof.
+    intros Hstar.
+    inv Hstar. reflexivity. inv H.
+  Qed.
+
+  Lemma trace_prefix' se s w t r:
+    lts_trace (Impl.lts σ L se) false (Impl.ext L s w) t r ->
+    exists t', t = w ++ t'.
+  Proof.
+    revert t. induction w.
+    - intros. eexists. reflexivity.
+    - intros t Hlts.
+      inv Hlts. inv H. inv H. inv H0.
+      inv H1. destruct w.
+      + eexists. cbn. reflexivity.
+      + eapply star_ext_state' in H.
+        subst. exploit IHw. eauto.
+        intros [? ?]. eexists.
+        rewrite <- app_comm_cons. f_equal. eauto.
+  Qed.
+
+  Let Lσ := Impl.semantics (skel L) σ L.
+  Lemma Lσ_coh: sem_coherence Lσ.
+  Proof.
+    intros se bot_tr' [q' r'] bot_tr [q r] H H0. cbn.
+    intros Hcoh. assert (q' = q -> r' = r /\ bot_tr' = bot_tr).
+    {
+      intros ->. inv H. inv H0. inv H5. inv H7.
+      exploit (sd_initial_determ (HL se)). apply H. apply H0.
+      intros ->. clear H H0 H2 H3.
+      revert bot_tr Hcoh H8. induction H6.
+      - intros tr Hcoh Hlts.
+        inv Hlts. apply IHlts_trace. auto.
+        replace s' with s'0. auto.
+        clear - Hcoh HL H H0 H1 H6. revert s'0 H0 H1.
+        induction H.
+        + intros. inv H0; auto.
+          inv H6.
+          * inv H0. inv H.
+            -- exploit (sd_final_nostep (HL se)); eauto. easy.
+            -- exploit (sd_final_noext (HL se)); eauto. easy.
+          * inv H0. inv H.
+        + intros. specialize (IHstar H6).
+          inv H2.
+          * inv H3.
+            -- inv H1. inv H.
+               ** exploit (sd_final_nostep (HL se)); eauto. easy.
+               ** exploit (sd_final_noext (HL se)); eauto. easy.
+            -- inv H1. inv H.
+          * inv H.
+            -- inv H4.
+               ** exploit (sd_determ (HL se)). apply H1. apply H2.
+                  exploit (sd_traces (HL se)). apply H1.
+                  exploit (sd_traces (HL se)). apply H2. intros l1 l2.
+                  intros [Hmt Ht].
+                  assert (t1 = t3 /\ t2 = t4).
+                  destruct t1. inv Hmt. split; auto.
+                  destruct t1. 2: { simpl in l2. try omegaContradiction. }
+                  destruct t3. inv Hmt. destruct t3.
+                  2: { simpl in l1. try omegaContradiction. }
+                  simpl in H7. inv H7. split; auto.
+                  exploit Ht. apply H. intros <-.
+                  destruct H as [<- <-].
+                  eapply IHstar. auto. auto.
+               ** exploit (sd_at_external_nostep (HL se)); eauto. easy.
+            -- inv H4.
+               ** exploit (sd_at_external_nostep (HL se)); eauto. easy.
+               ** exploit (sd_at_external_determ (HL se)). apply H1. apply H9.
+                  intros <-.
+                  destruct t0; destruct t1.
+               ++ pose proof (has_coh _ _ _ _ H8 H11).
+                  cbn in H. exploit H. constructor.
+                  intros [Hl Hqr]. exploit (proj2 Hl). auto. intros <-.
+                  exploit (sd_after_external_determ (HL se)). apply H2. apply H10.
+                  intros <-. simpl in H7. subst. apply IHstar. auto. auto.
+               ++ pose proof (has_coh _ _ _ _ H8 H11).
+                  cbn in H. exploit H. constructor.
+                  intros [Hl Hqr]. exploit (proj2 Hl). auto. intros <-.
+                  exploit Hqr. auto. intros. easy.
+               ++ pose proof (has_coh _ _ _ _ H8 H11).
+                  cbn in H. exploit H. constructor.
+                  intros [Hl Hqr]. exploit (proj2 Hl). auto. intros <-.
+                  exploit Hqr. constructor. intros. easy.
+               ++ pose proof (has_coh _ _ _ _ H8 H11).
+                  cbn in H. exploit H.
+                  exploit star_ext_state'. apply H0. intros ->.
+                  exploit star_ext_state'. apply H5. intros ->.
+                  exploit trace_prefix'. apply H6. intros [? ->].
+                  exploit trace_prefix'. apply H3. intros [? ->].
+                  eapply prefix_coh. eauto.
+                  intros [Hl Hqr]. exploit (proj2 Hl). auto. intros <-.
+                  exploit (sd_after_external_determ (HL se)). apply H2. apply H10.
+                  intros <-. simpl in H7. subst.
+                  exploit Hqr. auto. intros. inv H4.
+                  apply IHstar. auto. auto.
+            -- inv H4. simpl in H7. subst.
+               apply IHstar. auto. auto.
+      - intros tr Hcoh Hlts. inv Hcoh.
+        + inv H. inv Hlts.
+          * inv H. exploit (sd_final_determ (HL se)). apply H0. apply H2. easy.
+          * inv H.
+        + inv Hlts. inv H. inv H0.
+          exploit (sd_final_determ (HL se)). apply H1. apply H2. easy.
+      - intros tr Hcoh Hlts.
+        inv Hcoh.
+        + inv Hlts. inv H1. inv H.
+        + destruct b as [q' r'].
+          inv Hlts. inv H. inv H7.
+          inv H0. inv H9. exploit H5. auto.
+          intros Hcoh'.
+          exploit IHlts_trace; eauto. intros [<- <-]. easy.
+    }
+    intuition. apply H1. now injection H2.
+  Qed.
+
+  Program Definition hcomp_sem se: coh_semantics liA liC :=
+    {|
+    vq := valid_query (L se);
+    lf := compcerto_lmap' Lσ Lσ_coh se;
+    |}.
+  Next Obligation.
+    inv H. apply H2.
+  Qed.
+End IMPL_EMBED.
+Definition c_hcomp_sem p C se :=
+  hcomp_sem (fun se => clight_bigstep p se @ !li_dc)
+            (semantics1 C) (clight_determinate C) se.
